theories/Stlc/Symbolic/FreeReconstruct.v
@@ -56,7 +56,7 @@ Set Implicit Arguments.
     (at level 8, left associativity,
       format "s [ ζ ]").
 
-Section Generate.
+Section Implementation.
   Import MonadNotations.
   Import World.notations.
 
@@ -86,8 +86,8 @@ Section Generate.
           [ _ ] '(t2,e') <- gen e (Γ[_] ,, x∷t1) ;;
           Ret (ṫy.func t1[_] t2, ėxp.abst x t1[_] e')
       | exp.abst x t1 e =>
-          [ _ ] '(t2,e') <- gen e (Γ ,, x∷lift t1 _) ;;
-          Ret (ṫy.func (lift t1 _) t2, ėxp.abst x (lift t1 _) e')
+          [ _ ] '(t2,e') <- gen e (Γ ,, x∷lift t1) ;;
+          Ret (ṫy.func (lift t1) t2, ėxp.abst x (lift t1) e')
       | exp.app e1 e2 =>
           [ _ ] '(tf, e1') <- gen e1 Γ ;;
           [ _ ] '(t1, e2') <- gen e2 Γ[_] ;;
@@ -96,22 +96,18 @@ Section Generate.
           Ret (t2[_], ėxp.app e1'[_] e2'[_])
       end.
 
-End Generate.
-
-Section Reconstruct.
-
-  Definition reconstruct (G : Env) (e : Exp) :
+  Definition reconstruct (Γ : Env) (e : Exp) :
     option { w & Ṫy w * Ėxp w }%type :=
-    option.bind (prenex (generate e (lift G world.nil)))
+    option.bind (prenex (generate e (lift (w:=world.nil) Γ)))
       (fun '(existT w1 (_ , (C , te))) =>
           option.bind (solve C)
             (fun '(existT w2 (θ2 , _)) =>
                Some (existT w2 te[θ2]))).
 
-  Definition reconstruct_grounded G (e : Exp) : option (Ty * Exp) :=
-    option.map (fun '(existT w te) => inst te (grounding w)) (reconstruct G e).
+  Definition reconstruct_grounded (Γ : Env) (e : Exp) : option (Ty * Exp) :=
+    option.map (fun '(existT w te) => inst te (grounding w)) (reconstruct Γ e).
 
-End Reconstruct.
+End Implementation.
 
 Section Correctness.
 
@@ -173,7 +169,7 @@ Section Correctness.
       pred_unfold. psimplnew.
 
     - rewrite wlp_bind. unfold _4.
-      iPoseProof (IHe _ (G ,, x∷lift t w)) as "-#IH". iRevert "IH". clear IHe.
+      iPoseProof (IHe _ (G ,, x∷lift t)) as "-#IH". iRevert "IH". clear IHe.
       iApply (@wlp_mono alloc.acc_alloc). iIntros (w1 θ1 (t1 & e1')) "!> HT".
       predsimpl. iStopProof. pred_unfold. constructor. psimplnew.
     - rewrite wlp_bind. unfold _4.
@@ -197,9 +193,9 @@ Section Correctness.
 
   Lemma generate_complete_aux {G e t ee} (T : G |-- e ∷ t ~> ee) :
     forall w0 (G0 : Ėnv w0),
-      ⊢ lift G _ =ₚ G0 →
+      ⊢ lift G =ₚ G0 →
       WP (Θ := alloc.acc_alloc) (generate e G0)
-          (fun w1 r01 '(t',e') => lift t w1 =ₚ t' /\ₚ Sem.pure ee =ₚ e')%P.
+          (fun w1 r01 '(t',e') => lift t =ₚ t' /\ₚ Sem.pure ee =ₚ e')%P.
   Proof.
     induction T as [G x t Hres|G|G|G e1 e1' e2 e2' e3 e3' t _ IH1 _ IH2 _ IH3
       |G x t1 t2 e e' _ IH|G x t1 t2 e e' _ IH|G e1 t2 e1' e2 t1 e2' _ IH1 _ IH2];
@@ -225,7 +221,7 @@ Section Correctness.
       iStopProof. constructor. intros ι [_ [(HeqG & Heq1 & Heq2 & Heq3 & Heq4 & Heq5 & Heq6)]].
       pred_unfold. psimplnew.
 
-    - iIntros "#HeqG". rewrite Acc.intro_wp_step. iExists (lift t1 _). iIntros "!> #Heq1".
+    - iIntros "#HeqG". rewrite Acc.intro_wp_step. iExists (lift t1). iIntros "!> #Heq1".
       rewrite wp_bind. unfold _4. predsimpl.
       iPoseProof (IH _ (G0 ,, x∷ṫy.var world.in_zero)) as "IH". clear IH. predsimpl.
       iPoseProof ("IH" with "HeqG Heq1") as "-#IH'"; iClear "IH". iRevert "IH'".
@@ -237,7 +233,7 @@ Section Correctness.
 
     - iIntros "#HeqG".
       rewrite wp_bind. unfold _4.
-      iPoseProof (IH _ (G0 ,, x∷lift t1 w0)) as "IH". clear IH. predsimpl.
+      iPoseProof (IH _ (G0 ,, x∷lift t1)) as "IH". clear IH. predsimpl.
       iPoseProof ("IH" with "HeqG") as "-#IH'"; iClear "IH". iRevert "IH'".
       iApply (@wp_mono alloc.acc_alloc).
       iIntros (w1 r1 (t2' & e'')) "!> (#Heq1 & #Heq2)"; predsimpl.
@@ -256,42 +252,42 @@ Section Correctness.
       iPoseProof (IH2 w1 G0 with "HeqG") as "-#IH"; clear IH2. iRevert "IH".
       iApply (@wp_mono alloc.acc_alloc).
       iIntros (w2 r2 (t1' & e2'')) "!> (#Heq3 & #Heq4)"; predsimpl.
-      rewrite Acc.intro_wp_step. iExists (lift t2 w2). unfold _4. predsimpl.
+      rewrite Acc.intro_wp_step. iExists (lift t2). unfold _4.
       iIntros "!>". predsimpl.
 
       iStopProof. constructor. intros ι [_ [(HeqG & Heq1 & Heq2 & Heq3 & Heq4)]].
       pred_unfold. psimplnew.
   Qed.
 
-  Lemma generate_complete (e : Exp) (w0 : World) (G0 : Ėnv w0) t0 e0 :
-    G0 |--ₚ e; t0 ~> e0 ⊢ₚ TPB_algo G0 e t0 e0.
+  Lemma generate_complete  {w} (Γ : Ėnv w) (e : Exp) (τ : Ṫy w) (e' : Ėxp w) :
+    Γ |--ₚ e; τ ~> e' ⊢ₚ TPB_algo Γ e τ e'.
   Proof.
     constructor. intros ι HT.
-    destruct (@generate_complete_aux _ _ _ _ HT w0 G0) as [Hcompl].
+    destruct (generate_complete_aux HT Γ) as [Hcompl].
     specialize (Hcompl ι (MkEmp _)). pred_unfold.
     specialize (Hcompl eq_refl). revert Hcompl.
-    apply wp_mono. intros w1 θ1 [t1 e1]. cbn.
+    apply wp_mono. intros w1 θ1 [τ1 e1]. cbn.
     intros ι1 <-. pred_unfold. psimplnew.
   Qed.
 
-  Lemma generate_correct (e : Exp) (w0 : World) (G0 : Ėnv w0) t0 e0 :
-    G0 |--ₚ e; t0 ~> e0 ⊣⊢ₚ TPB_algo G0 e t0 e0.
-  Proof. apply split_bientails. auto using generate_complete, generate_sound. Qed.
+  Lemma generate_correct {w} (Γ : Ėnv w) (e : Exp) (τ : Ṫy w) (e' : Ėxp w) :
+    Γ |--ₚ e; τ ~> e' ⊣⊢ₚ TPB_algo Γ e τ e'.
+  Proof. apply split_bientails; auto using generate_complete, generate_sound. Qed.
 
   Import (hints) Acc.
 
-  Definition tpb_algo (G : Env) (e : Exp) (t : Ty) (ee : Exp) : Prop :=
-    match reconstruct G e with
-    | Some (existT w (t', ee')) =>
-        exists ι : Assignment w, inst t' ι = t /\ inst ee' ι = ee
+  Definition algorithmic_typing (Γ : Env) (e : Exp) (τ : Ty) (e' : Exp) : Prop :=
+    match reconstruct Γ e with
+    | Some (existT w1 (τ1, e1)) =>
+        exists ι : Assignment w1, inst τ1 ι = τ /\ inst e1 ι = e'
     | None => False
     end.
 
-  Lemma correctness (G : Env) (e : Exp) (t : Ty) (ee : Exp) :
-    tpb G e t ee <-> tpb_algo G e t ee.
+  Lemma correctness (Γ : Env) (e : Exp) (τ : Ty) (e' : Exp) :
+    algorithmic_typing Γ e τ e' <-> tpb Γ e τ e'.
   Proof.
-    generalize (generate_correct e (lift G world.nil) (lift t _) (lift ee _)).
-    unfold TPB_algo, tpb_algo, reconstruct. rewrite <- prenex_correct.
+    generalize (generate_correct (w:=world.nil) (lift Γ) e (lift τ) (lift e')).
+    unfold TPB_algo, algorithmic_typing, reconstruct. rewrite <- prenex_correct.
     destruct prenex as [(w1 & θ1 & C & t1 & e1)|]; cbn.
     - rewrite <- (solve_correct C).
       destruct (solve C) as [(w2 & θ2 & [])|]; predsimpl.
@@ -299,11 +295,11 @@ Section Correctness.
         intros [HE]. specialize (HE env.nil). pred_unfold.
         rewrite HE. clear HE. unfold Acc.wp.
         split.
-        * intros (ι1 & Heq1 & ι2 & Heq2 & Heq3 & Heq4).
-          exists ι2. now pred_unfold.
         * intros (ι2 & Heq1 & Heq2). exists (inst θ2 ι2).
           split; [now destruct (env.view (inst θ1 (inst θ2 ι2)))|].
           exists ι2. subst. now pred_unfold.
+        * intros (ι1 & Heq1 & ι2 & Heq2 & Heq3 & Heq4).
+          exists ι2. now pred_unfold.
       + intros [HE]. specialize (HE env.nil). now pred_unfold.
     - intros [HE]. specialize (HE env.nil). now pred_unfold.
   Qed.
